SEARllist.sml
@@ -467,12 +467,6 @@ cheat
 *)
 
 
-val tof_Tpm_inv = prove_store("tof_Tpm_inv",
-e0
-(rpt strip_tac >> rw[GSYM FUN_EXT] >>
- rw[GSYM tof_def,Tpm_def])
-(form_goal
- “!A B f:A->B. tof(Tpm(f))  = f”));
 
 
 (*FUNPOW*)
