SEARpred_set.sml
@@ -1,0 +1,13 @@
+
+val tof_Tpm_inv = prove_store("tof_Tpm_inv",
+e0
+(rpt strip_tac >> rw[GSYM FUN_EXT] >>
+ rw[GSYM tof_def,Tpm_def])
+(form_goal
+ “!A B f:A->B. tof(Tpm(f))  = f”));
+
+
+val IN_Sing = prove_store("IN_Sing",
+e0
+(rw[Sing_def,Sg_def])
+(form_goal “!A a0 a:mem(A). IN(a,Sing(a0)) <=> a = a0”));
